src/Zulib/verify.sh
@@ -1,0 +1,9 @@
+#!/bin/sh
+
+mono ../../packages/ZFStar/tools/fstar.exe \
+     --smt ../../packages/zen_z3_linux/output/z3-linux \
+     --prims fstar/prims.fst \
+     --no_default_includes \
+     --include ~/Dev/zenprotocol/src/Zulib/fstar \
+     --cache_checked_modules \
+     $@
